ulib/FStar.Pointer.Derived2.fst
@@ -1,0 +1,102 @@
+module FStar.Pointer.Derived2
+
+module DM = FStar.DependentMap
+module HH = FStar.HyperHeap
+module HS = FStar.HyperStack
+module HST = FStar.HyperStack.ST
+
+private
+let copy_buffer_contents_inv
+  (#t: typ)
+  (a: buffer t) (* source *)
+  (idx_a: UInt32.t)
+  (b: buffer t) (* destination *)
+  (idx_b: UInt32.t)
+  (len: UInt32.t)
+  (len' : UInt32.t)
+  (h: HS.mem)
+  (h' : HS.mem)
+: GTot Type0
+= copy_buffer_contents_precond a idx_a b idx_b len h /\
+  modifies (loc_buffer (gsub_buffer b idx_b len)) h h' /\
+  UInt32.v len' <= UInt32.v len /\
+  buffer_readable h' (gsub_buffer b idx_b len') /\
+  buffer_as_seq h' (gsub_buffer b idx_b len') == buffer_as_seq h (gsub_buffer a idx_a len')
+
+private
+assume
+val copy_buffer_contents_init
+  (#t: typ)
+  (a: buffer t) (* source *)
+  (idx_a: UInt32.t)
+  (b: buffer t) (* destination *)
+  (idx_b: UInt32.t)
+  (len: UInt32.t)
+  (h: HS.mem)
+: Lemma
+  (requires (copy_buffer_contents_precond a idx_a b idx_b len h))
+  (ensures (copy_buffer_contents_inv a idx_a b idx_b len 0ul h h))
+
+(*
+= buffer_readable_intro_empty h (gsub_buffer b idx_b 0ul);
+  Seq.lemma_eq_intro (buffer_as_seq h (gsub_buffer b idx_b 0ul)) (buffer_as_seq h (gsub_buffer a idx_a 0ul))
+*)
+
+private
+assume
+val copy_buffer_contents_advance
+  (#t: typ)
+  (a: buffer t) (* source *)
+  (idx_a: UInt32.t)
+  (b: buffer t) (* destination *)
+  (idx_b: UInt32.t)
+  (len: UInt32.t)  
+  (len' : UInt32.t)
+  (h: Ghost.erased HS.mem)
+: HST.Stack unit
+  (requires (fun h0 ->
+    copy_buffer_contents_inv a idx_a b idx_b len len' (Ghost.reveal h) h0 /\
+    UInt32.v len' < UInt32.v len
+  ))
+  (ensures (fun h1 _ h2 ->
+    copy_buffer_contents_inv a idx_a b idx_b len len' (Ghost.reveal h) h1 /\
+    UInt32.v len' < UInt32.v len /\
+    copy_buffer_contents_inv a idx_a b idx_b len (UInt32.add len' 1ul) (Ghost.reveal h) h2
+  ))
+
+private
+assume
+val copy_buffer_contents_aux
+  (#t: typ)
+  (a: buffer t) (* source *)
+  (idx_a: UInt32.t)
+  (b: buffer t) (* destination *)
+  (idx_b: UInt32.t)
+  (len: UInt32.t)
+  (len': UInt32.t)
+  (h: Ghost.erased HS.mem)
+: HST.Stack unit
+  (requires (fun h0 ->
+    copy_buffer_contents_inv a idx_a b idx_b len len' (Ghost.reveal h) h0
+  ))
+  (ensures (fun h0 _ h1 ->
+    copy_buffer_contents_inv a idx_a b idx_b len len' (Ghost.reveal h) h0 /\
+    copy_buffer_contents_postcond a idx_a b idx_b len (Ghost.reveal h) h1
+  ))
+//  (decreases (UInt32.v len - UInt32.v len'))
+
+(*
+let rec copy_buffer_contents_aux #t a idx_a b idx_b len len' h =
+  if len = len'
+  then ()
+  else begin
+    copy_buffer_contents_advance a idx_a b idx_b len len' h;
+    copy_buffer_contents_aux a idx_a b idx_b len (UInt32.add len' 1ul) h
+  end
+*)
+
+let copy_buffer_contents #t a idx_a b idx_b len =
+  let h0 = HST.get () in
+  copy_buffer_contents_init a idx_a b idx_b len h0;
+  copy_buffer_contents_aux a idx_a b idx_b len 0ul (Ghost.hide h0);
+  admit ()
